SStructTT/SStruct/Syntax.lean
@@ -13,10 +13,10 @@ inductive Tm where
   | srt (s : Srt) (i : Nat)
   | pi  (A B : Tm) (r : Rlv) (s : Srt)
   | lam (A m : Tm) (r : Rlv) (s : Srt)
-  | app (m n : Tm) (r : Rlv)
+  | app (m n : Tm)
   | sig (A B : Tm) (r : Rlv) (s : Srt)
   | tup (m n : Tm) (r : Rlv) (s : Srt)
-  | prj (A m n : Tm) (r : Rlv)
+  | prj (A m n : Tm)
   | bool | tt | ff
   | ite (A m n1 n2 : Tm)
   | idn (A m n : Tm)
@@ -36,10 +36,10 @@ def rename_rec (ξ : Var -> Var) (m : Tm Srt) : Tm Srt :=
   | srt s i => srt s i
   | pi A B r s => pi (rename_rec ξ A) (rename_rec (upren ξ) B) r s
   | lam A m r s => lam (rename_rec ξ A) (rename_rec (upren ξ) m) r s
-  | app m n r => app (rename_rec ξ m) (rename_rec ξ n) r
+  | app m n => app (rename_rec ξ m) (rename_rec ξ n)
   | sig A B r s => sig (rename_rec ξ A) (rename_rec (upren ξ) B) r s
   | tup m n r s => tup (rename_rec ξ m) (rename_rec ξ n) r s
-  | prj A m n r => prj (rename_rec (upren ξ) A) (rename_rec ξ m) (rename_rec (upren $ upren ξ) n) r
+  | prj A m n => prj (rename_rec (upren ξ) A) (rename_rec ξ m) (rename_rec (upren $ upren ξ) n)
   | bool => bool
   | tt => tt
   | ff => ff
@@ -58,10 +58,10 @@ variable (ξ : Var -> Var) (A B m n n1 n2 : Tm Srt) (x i : Nat) (r : Rlv) (s : S
 @[asimp]lemma srt  : rename ξ (srt s i) = srt s i := by rfl
 @[asimp]lemma pi   : rename ξ (pi A B r s) = pi (rename ξ A) (rename (upren ξ) B) r s := by rfl
 @[asimp]lemma lam  : rename ξ (lam A m r s) = lam (rename ξ A) (rename (upren ξ) m) r s := by rfl
-@[asimp]lemma app  : rename ξ (app m n r) = app (rename ξ m) (rename ξ n) r := by rfl
+@[asimp]lemma app  : rename ξ (app m n) = app (rename ξ m) (rename ξ n) := by rfl
 @[asimp]lemma sig1 : rename ξ (sig A B r s) = sig (rename ξ A) (rename (upren ξ) B) r s := by rfl
 @[asimp]lemma tup1 : rename ξ (tup m n r s) = tup (rename ξ m) (rename ξ n) r s := by rfl
-@[asimp]lemma prj : rename ξ (prj A m n r) = prj (rename (upren ξ) A) (rename ξ m) (rename (upren $ upren ξ) n) r := by rfl
+@[asimp]lemma prj : rename ξ (prj A m n) = prj (rename (upren ξ) A) (rename ξ m) (rename (upren $ upren ξ) n) := by rfl
 @[asimp]lemma bool : rename ξ (@bool Srt) = bool := by rfl
 @[asimp]lemma tt   : rename ξ (@tt Srt) = tt := by rfl
 @[asimp]lemma ff   : rename ξ (@ff Srt) = ff := by rfl
@@ -78,10 +78,10 @@ def subst_rec (σ : Var -> Tm Srt) (m : Tm Srt) : Tm Srt :=
   | srt s i => srt s i
   | pi A B r s => pi (subst_rec σ A) (subst_rec (up σ) B) r s
   | lam A m r s => lam (subst_rec σ A) (subst_rec (up σ) m) r s
-  | app m n r => app (subst_rec σ m) (subst_rec σ n) r
+  | app m n => app (subst_rec σ m) (subst_rec σ n)
   | sig A B r s => sig (subst_rec σ A) (subst_rec (up σ) B) r s
   | tup m n r s => tup (subst_rec σ m) (subst_rec σ n) r s
-  | prj A m n r => prj (subst_rec (up σ) A) (subst_rec σ m) (subst_rec (upn 2 σ) n) r
+  | prj A m n => prj (subst_rec (up σ) A) (subst_rec σ m) (subst_rec (upn 2 σ) n)
   | bool => bool
   | tt => tt
   | ff => ff
@@ -100,10 +100,10 @@ variable (σ : Var -> Tm Srt) (A B m n n1 n2 : Tm Srt) (x i : Nat) (r : Rlv) (s 
 @[asimp]lemma srt  : subst σ (srt s i) = srt s i := by rfl
 @[asimp]lemma pi   : subst σ (pi A B r s) = pi (subst σ A) (subst (up σ) B) r s := by rfl
 @[asimp]lemma lam  : subst σ (lam A m r s) = lam (subst σ A) (subst (up σ) m) r s := by rfl
-@[asimp]lemma app  : subst σ (app m n r) = app (subst σ m) (subst σ n) r := by rfl
+@[asimp]lemma app  : subst σ (app m n) = app (subst σ m) (subst σ n) := by rfl
 @[asimp]lemma sig  : subst σ (sig A B r s) = sig (subst σ A) (subst (up σ) B) r s := by rfl
 @[asimp]lemma tup  : subst σ (tup m n r s) = tup (subst σ m) (subst σ n) r s := by rfl
-@[asimp]lemma prj : subst σ (prj A m n r) = prj (subst (up σ) A) (subst σ m) (subst (upn 2 σ) n) r := by rfl
+@[asimp]lemma prj : subst σ (prj A m n) = prj (subst (up σ) A) (subst σ m) (subst (upn 2 σ) n) := by rfl
 @[asimp]lemma bool : subst σ (@bool Srt) = bool := by rfl
 @[asimp]lemma tt   : subst σ (@tt Srt) = tt := by rfl
 @[asimp]lemma ff   : subst σ (@ff Srt) = ff := by rfl
@@ -125,10 +125,10 @@ lemma rename_subst ξ (m : Tm Srt) : rename ξ m = m.[ren ξ] := by
   | srt => asimp
   | pi A B r s ihA ihB => asimp[up_upren, ihA, ihB]
   | lam A m r s ihA ihm => asimp[up_upren, ihA, ihm]
-  | app m n r ihm ihn => asimp[ihm, ihn]
+  | app m n ihm ihn => asimp[ihm, ihn]
   | sig A B r s ihA ihB => asimp[up_upren, ihA, ihB]
   | tup m n r s ihm ihn => asimp[ihm, ihn]
-  | prj A m n r ihA ihm ihn => asimp[up_upren, ihm, ihA, ihn]
+  | prj A m n ihA ihm ihn => asimp[up_upren, ihm, ihA, ihn]
   | bool => asimp
   | tt => asimp
   | ff => asimp
@@ -149,10 +149,10 @@ lemma subst_id (m : Tm Srt) : m.[ids] = m := by
   | srt => asimp
   | pi A B r s ihA ihB => asimp[up_ids, ihA, ihB]
   | lam A m r s ihA ihm => asimp[up_ids, ihA, ihm]
-  | app m n r ihm ihn => asimp[ihm, ihn]
+  | app m n ihm ihn => asimp[ihm, ihn]
   | sig A B r s ihA ihB => asimp[up_ids, ihA, ihB]
   | tup m n r s ihm ihn => asimp[ihm, ihn]
-  | prj A m n r ihA ihm ihn => asimp[up_ids, ihm, ihA, ihn]
+  | prj A m n ihA ihm ihn => asimp[up_ids, ihm, ihA, ihn]
   | bool => asimp
   | tt => asimp
   | ff => asimp
@@ -174,10 +174,10 @@ lemma ren_subst_comp ξ σ (m : Tm Srt) : m.[ren ξ].[σ] = m.[ξ !>> σ] := by
   | srt => asimp
   | pi A B r s ihA ihB => asimp[up_upren, up_comp_upren, ihA, ihB]
   | lam A m r s ihA ihm => asimp[up_upren, up_comp_upren, ihA, ihm]
-  | app m n r ihm ihn => asimp[ihm, ihn]
+  | app m n ihm ihn => asimp[ihm, ihn]
   | sig A B r s ihA ihB => asimp[up_upren, up_comp_upren, ihA, ihB]
   | tup m n r s ihm ihn => asimp[ihm, ihn]
-  | prj A m n r ihA ihm ihn => asimp[up_upren, up_comp_upren, ihm, ihA, ihn]
+  | prj A m n ihA ihm ihn => asimp[up_upren, up_comp_upren, ihm, ihA, ihn]
   | bool => asimp
   | tt => asimp
   | ff => asimp
@@ -203,10 +203,10 @@ lemma subst_ren_comp σ ξ (m : Tm Srt) : m.[σ].[ren ξ] = m.[σ !>> rename ξ]
   | srt => asimp
   | pi A B r s ihA ihB => asimp[up_upren, up_comp_ren, ihA, ihB]
   | lam A m r s ihA ihm => asimp[up_upren, up_comp_ren, ihA, ihm]
-  | app m n r ihm ihn => asimp[ihm, ihn]
+  | app m n ihm ihn => asimp[ihm, ihn]
   | sig A B r s ihA ihB => asimp[up_upren, up_comp_ren, ihA, ihB]
   | tup m r n s ihm ihn => asimp[ihm, ihn]
-  | prj A m n r ihA ihm ihn => asimp[up_upren, up_comp_ren, ihm, ihA, ihn]
+  | prj A m n ihA ihm ihn => asimp[up_upren, up_comp_ren, ihm, ihA, ihn]
   | bool => asimp
   | tt => asimp
   | ff => asimp
@@ -232,10 +232,10 @@ lemma subst_comp (σ τ : Var -> Tm Srt) m : m.[σ].[τ] = m.[σ !> τ] := by
   | srt => asimp
   | pi A B r s ihA ihB => asimp[up_comp, ihA, ihB]
   | lam A m r s ihA ihm => asimp[up_comp, ihA, ihm]
-  | app m n r ihm ihn => asimp[ihm, ihn]
+  | app m n ihm ihn => asimp[ihm, ihn]
   | sig A B r s ihA ihB => asimp[up_comp, ihA, ihB]
   | tup m n r s ihm ihn => asimp[ihm, ihn]
-  | prj A m n r ihA ihm ihn => asimp[up_comp, ihm, ihA, ihn]
+  | prj A m n ihA ihm ihn => asimp[up_comp, ihm, ihA, ihn]
   | bool => asimp
   | tt => asimp
   | ff => asimp
