SStructTT/SStruct/Dynamic/Step.lean
@@ -23,20 +23,17 @@ inductive Value : Tm Srt -> Prop where
 
 @[scoped aesop safe [constructors]]
 inductive Step : Tm Srt -> Tm Srt -> Prop where
-  | app_im_M {m m'} n :
+  | app_M {m m'} n :
     Step m m' ->
-    Step (.app m n .im) (.app m' n .im)
-  | app_ex_M {m m'} n :
-    Step m m' ->
-    Step (.app m n .ex) (.app m' n .ex)
-  | app_ex_N m {n n'} :
+    Step (.app m n) (.app m' n)
+  | app_N m {n n'} :
     Step n n' ->
-    Step (.app m n .ex) (.app m n' .ex)
+    Step (.app m n) (.app m n')
   | beta_im A m n s :
-    Step (.app (.lam A m .im s) n .im) m.[n/]
+    Step (.app (.lam A m .im s) n) m.[n/]
   | beta_ex A m n s :
     Value n ->
-    Step (.app (.lam A m .ex s) n .ex) m.[n/]
+    Step (.app (.lam A m .ex s) n) m.[n/]
   | tup_im_N m {n n'} s :
     Step n n' ->
     Step (.tup m n .im s) (.tup m n' .im s)
@@ -46,18 +43,15 @@ inductive Step : Tm Srt -> Tm Srt -> Prop where
   | tup_ex_N m {n n'} s :
     Step n n' ->
     Step (.tup m n .ex s) (.tup m n' .ex s)
-  | prj_im_M A {m m'} n :
+  | prj_M A {m m'} n :
     Step m m' ->
-    Step (.prj A m n .im) (.prj A m' n .im)
-  | prj_ex_M A {m m'} n :
-    Step m m' ->
-    Step (.prj A m n .ex) (.prj A m' n .ex)
+    Step (.prj A m n) (.prj A m' n)
   | prj_im_elim A {m1 m2} n {s} :
     Value (.tup m1 m2 .im s) ->
-    Step (.prj A (.tup m1 m2 .im s) n .im) n.[m2,m1/]
+    Step (.prj A (.tup m1 m2 .im s) n) n.[m2,m1/]
   | prj_ex_elim A {m1 m2} n {s} :
     Value (.tup m1 m2 .ex s) ->
-    Step (.prj A (.tup m1 m2 .ex s) n .ex) n.[m2,m1/]
+    Step (.prj A (.tup m1 m2 .ex s) n) n.[m2,m1/]
   | ite_M A {m m'} n1 n2 :
     Step m m' ->
     Step (.ite A m n1 n2) (.ite A m' n1 n2)
@@ -72,14 +66,10 @@ notation:50 m:50 " ~>> " n:50 => Step m n
 notation:50 m:50 " ~>>* " n:50 => ARS.Star Step m n
 notation:50 m:50 " ~>>1 " n:50 => ARS.Star1 Step m n
 
-lemma Red.app_im {m m' n : Tm Srt} :
-    m ~>>* m' -> .app m n .im ~>>* .app m' n .im := by
-  intro rm; apply Star.hom _ _ rm; aesop
-
-lemma Red.app_ex {m m' n n' : Tm Srt} :
-    m ~>>* m' -> n ~>>* n' -> .app m n .ex ~>>* .app m' n' .ex := by
+lemma Red.app {m m' n n' : Tm Srt} :
+    m ~>>* m' -> n ~>>* n' -> .app m n ~>>* .app m' n' := by
   intro rm rn;
-  apply @Star.trans _ _ (.app m' n .ex)
+  apply @Star.trans _ _ (.app m' n)
   apply Star.hom _ _ rm; aesop
   apply Star.hom _ _ rn; aesop
 
@@ -94,24 +84,20 @@ lemma Red.tup_ex {m m' n n' : Tm Srt} {s} :
   apply Star.hom _ _ rm; aesop
   apply Star.hom _ _ rn; aesop
 
-lemma Red.prj {A m m' n : Tm Srt} {r} :
-    m ~>>* m' -> .prj A m n r ~>>* .prj A m' n r := by
-  intro rm; apply Star.hom _ _ rm; cases r <;> aesop
+lemma Red.prj {A m m' n : Tm Srt} :
+    m ~>>* m' -> .prj A m n ~>>* .prj A m' n := by
+  intro rm; apply Star.hom _ _ rm; aesop
 
 lemma Red.ite {A m m' n1 n2 : Tm Srt} :
     m ~>>* m' -> .ite A m n1 n2 ~>>* .ite A m' n1 n2 := by
   intro rm; apply Star.hom _ _ rm; aesop
 
-lemma Red1.app_im {m m' n : Tm Srt} :
-    m ~>>1 m' -> .app m n .im ~>>1 .app m' n .im := by
+lemma Red1.app_M {m m' n : Tm Srt} :
+    m ~>>1 m' -> .app m n ~>>1 .app m' n := by
   intro rm; apply Star1.hom _ _ rm; aesop
 
-lemma Red1.app_ex_M {m m' n : Tm Srt} :
-    m ~>>1 m' -> .app m n .ex ~>>1 .app m' n .ex := by
-  intro rm; apply Star1.hom _ _ rm; aesop
-
-lemma Red1.app_ex_N {m n n' : Tm Srt} :
-    n ~>>1 n' -> .app m n .ex ~>>1 .app m n' .ex := by
+lemma Red1.app_N {m n n' : Tm Srt} :
+    n ~>>1 n' -> .app m n ~>>1 .app m n' := by
   intro rn; apply Star1.hom _ _ rn; aesop
 
 lemma Red1.tup_im {m n n' : Tm Srt} {s} :
@@ -126,9 +112,9 @@ lemma Red1.tup_ex_N {m n n' : Tm Srt} {s} :
     n ~>>1 n' -> .tup m n .ex s ~>>1 .tup m n' .ex s := by
   intro rn; apply Star1.hom _ _ rn; aesop
 
-lemma Red1.prj {A m m' n : Tm Srt} {r} :
-    m ~>>1 m' -> .prj A m n r ~>>1 .prj A m' n r := by
-  intro rm; apply Star1.hom _ _ rm; cases r <;> aesop
+lemma Red1.prj {A m m' n : Tm Srt} :
+    m ~>>1 m' -> .prj A m n ~>>1 .prj A m' n := by
+  intro rm; apply Star1.hom _ _ rm; aesop
 
 lemma Red1.ite {A m m' n1 n2 : Tm Srt} :
     m ~>>1 m' -> .ite A m n1 n2 ~>>1 .ite A m' n1 n2 := by
